theories/lam/lib/fixlam.v
@@ -1,22 +1,104 @@
-From st.lam Require Export types lang typing.
+From st.lam Require Import types lang tactics typing.
 
 Local Open Scope expr_no_st_scope.
 Local Open Scope types_no_st_scope.
 
-Definition FixLam (e : expr) : expr :=
-  (Rec (e.[upn 1 (ren (+2))].[%0 %1/]) (Lam e)).
+Definition FixArrow (f : expr) : expr :=
+  Unfold (Fold (Lam ((f.[ren (+1)]) (Lam ((Unfold (Var 1)) (Var 1) (Var 0))))))
+    (Fold (Lam (f.[ren (+1)] (Lam ((Unfold (Var 1)) (Var 1) (Var 0)))))).
 
-Lemma FixLam_typed Γ e τ (d : τ :: Γ ⊢ₙₒ e : τ) : Γ ⊢ₙₒ FixLam e : τ.
+Lemma FixArrow_subst e σ : (FixArrow e).[σ] = FixArrow e.[σ].
+Proof. rewrite /FixArrow. by asimpl. Qed.
+
+Lemma help τ1 τ2 : (TRec (TVar 0 ⟶ τ1.[ren (+1)] ⟶ τ2.[ren (+1)]) ⟶ τ1 ⟶ τ2)%Tₙₒ = (TVar 0 ⟶ τ1.[ren (+1)] ⟶ τ2.[ren (+1)]).[TRec (TVar 0 ⟶ τ1.[ren (+1)] ⟶ τ2.[ren (+1)])%Tₙₒ/].
+Proof. by asimpl. Qed.
+
+Lemma FixArrow_typed Γ τ1 τ2 f : (Γ ⊢ₙₒ f : TArrow (TArrow τ1 τ2) (TArrow τ1 τ2))
+  -> (Γ ⊢ₙₒ FixArrow f : TArrow τ1 τ2).
 Proof.
-  apply App_typed with (τ1 := τ ⟶ τ); try by repeat econstructor. apply Rec_typed.
-  apply typed_subst with (τ2 := τ); try by repeat econstructor.
-  change ([τ] ++ (τ ⟶ τ) ⟶ τ :: τ ⟶ τ :: [] ++ Γ ⊢ₙₒ e.[upn 1 (ren (+2))] : τ).
-  by apply (context_gen_weakening ((τ ⟶ τ) ⟶ τ :: τ ⟶ τ :: [])).
+  intro df. apply App_typed with (τ1 := (TRec (TVar 0 ⟶ τ1.[ren (+1)] ⟶ τ2.[ren (+1)]))%Tₙₒ).
+  rewrite help. apply Unfold_typed. apply Fold_typed. apply Lam_typed. apply App_typed with (τ1 := TArrow τ1 τ2). asimpl.
+  change ([ TRec (TVar 0 ⟶ τ1.[ren (+1)] ⟶ τ2.[ren (+1)]) ] ++ Γ ⊢ₙₒ f.[ren (+ length [ TRec (TVar 0 ⟶ τ1.[ren (+1)] ⟶ τ2.[ren (+1)]) ])] : ((τ1 ⟶ τ2) ⟶ τ1 ⟶ τ2)%Tₙₒ). by apply context_weakening.
+  asimpl. apply Lam_typed. eapply App_typed. econstructor. erewrite help. apply Unfold_typed. by constructor. by constructor. by constructor.
+  apply Fold_typed. apply Lam_typed. apply App_typed with (τ1 := TArrow τ1 τ2). asimpl.
+  change ([ TRec (TVar 0 ⟶ τ1.[ren (+1)] ⟶ τ2.[ren (+1)]) ] ++ Γ ⊢ₙₒ f.[ren (+ length [ TRec (TVar 0 ⟶ τ1.[ren (+1)] ⟶ τ2.[ren (+1)]) ])] : ((τ1 ⟶ τ2) ⟶ τ1 ⟶ τ2)%Tₙₒ). by apply context_weakening.
+  asimpl. apply Lam_typed. eapply App_typed. econstructor. erewrite help. apply Unfold_typed. by constructor. by constructor. by constructor.
 Qed.
 
-Lemma FixLam_step σ κ e : prim_step (FixLam e) σ κ (e.[FixLam e/]) σ [].
+Lemma FixArrow_eval f : nsteps lam_step 2 (FixArrow f) (f (Lam ((FixArrow f).[ren (+1)] %0)))%Eₙₒ.
+Proof. do 2 (eapply nsteps_l; first auto_lam_step; asimpl). by apply nsteps_O. Qed.
+
+Definition FixLamBodyHelp (e : expr) := Lam ((Lam (e.[(%0 ())%Eₙₒ .: ren (+1)].[ren (+1)]))).
+
+Definition FixLam (e : expr) :=
+  (Lam ((FixArrow (FixLamBodyHelp e)).[ren (+1)] %0) ())%Eₙₒ.
+
+Lemma FixLam_eval e : nsteps lam_step 5 (FixLam e) (e.[FixLam e/]).
 Proof.
-  apply head_prim_step. rewrite /FixLam.
-  assert (e.[Rec e.[upn 1 (ren (+2))].[%0 %1/] (Lam e)/] = e.[upn 1 (ren (+2))].[%0 %1/].[Rec (e.[upn 1 (ren (+2))].[%0 %1/]),(Lam e)/]) as ->. by asimpl.
-  by eapply BetaS.
+  eapply nsteps_l. apply head_prim_step. auto_head_step.
+  cut (nsteps lam_step 4 ((FixArrow (FixLamBodyHelp e)) ()) e.[FixLam e/])%Eₙₒ. asimpl.
+  rewrite /FixArrow. by asimpl.
+  assert (4 = (2 + 2)%nat) as ->. done.
+  eapply nsteps_trans.
+  eapply (nsteps_congruence (fill [AppLCtx ()%Eₙₒ])). intros. apply lam_step_ctx. apply ectx_lang_ctx. apply H.
+  apply FixArrow_eval.
+  eapply nsteps_l. auto_lam_step. asimpl.
+  eapply nsteps_l. auto_lam_step. asimpl.
+  rewrite /FixLam /FixLamBodyHelp. asimpl. apply nsteps_O.
 Qed.
+
+Lemma small_help Γ e τ i :
+  Γ ⊢ₙₒ e : τ → (alter (fun τ => TArrow TUnit τ) i Γ) ⊢ₙₒ e.[upn i ((%0 ())%Eₙₒ .: ren (+1))] : τ.
+Proof.
+  generalize dependent i.
+  generalize dependent τ.
+  generalize dependent Γ.
+  induction e; intros; simpl.
+  - destruct (iter_up_cases x i ((%0)%Eₙₒ ()%Eₙₒ .: ren (+1))) as [[-> lt] | [j [-> ->]]].
+    + inversion_clear H. constructor. rewrite list_lookup_alter_ne. auto. lia.
+    + inversion_clear H. destruct j. asimpl.
+      econstructor. econstructor. rewrite list_lookup_alter.
+      assert ((i + 0)%nat = i) as eq. lia. rewrite eq in H0.
+      by simplify_option_eq.
+      econstructor.
+      asimpl. constructor. rewrite list_lookup_alter_ne.
+      assert ((i + S j)%nat = S (i + j)%nat) as eq. lia. by rewrite eq in H0. lia.
+  - simpl. inversion_clear H. econstructor. eapply (IHe0 (τ1 :: Γ) τ (S i) H0). by eapply IHe.
+  - simpl. inversion_clear H. econstructor. eapply (IHe (τ1 :: Γ) τ2 (S i) H0).
+  - simpl. inversion_clear H. econstructor. by eapply IHe1. by eapply IHe2.
+  - simpl. inversion_clear H; econstructor.
+  - simpl. inversion_clear H. econstructor. by eapply IHe1. by eapply IHe2.
+  - simpl. inversion_clear H. econstructor. by eapply IHe1. by eapply IHe2. by eapply IHe3.
+  - simpl. inversion_clear H. econstructor. by eapply IHe1. by eapply IHe2.
+  - simpl. inversion_clear H. econstructor. by eapply IHe1. by eapply IHe2.
+  - simpl. inversion_clear H. econstructor. by eapply IHe.
+  - simpl. inversion_clear H. econstructor. by eapply IHe.
+  - simpl. inversion_clear H. econstructor. by eapply IHe.
+  - simpl. inversion_clear H. econstructor. by eapply IHe.
+  - simpl. inversion_clear H. econstructor. by eapply IHe.
+      by eapply (IHe0 (τ1 :: Γ) τ (S i)).
+      by eapply (IHe1 (τ2 :: Γ) τ (S i)).
+  - simpl. inversion_clear H. econstructor. by eapply IHe.
+  - simpl. inversion_clear H. econstructor. by eapply IHe.
+Qed.
+
+Lemma FixLamBodyHelp_typed Γ e τ : τ :: Γ ⊢ₙₒ e : τ → Γ ⊢ₙₒ FixLamBodyHelp e : ((TUnit ⟶ τ) ⟶ TUnit ⟶ τ)%Tₙₒ.
+Proof.
+  intro H.
+  apply Lam_typed. apply Lam_typed. change ([TUnit] ++ TUnit ⟶ τ :: Γ ⊢ₙₒ e.[%0 () .: ren (+1)].[ren (+1)] : τ). apply context_weakening.
+  cut ((alter (fun τ => TArrow TUnit τ) 0 (τ :: Γ)) ⊢ₙₒ e.[upn 0 ((%0 ())%Eₙₒ .: ren (+1))] : τ). by asimpl. by apply small_help.
+Qed.
+
+Lemma FixLam_typed Γ e τ : τ :: Γ ⊢ₙₒ e : τ → Γ ⊢ₙₒ FixLam e : τ.
+Proof.
+  intro H. apply App_typed with (τ1 := TUnit).
+  apply Lam_typed. apply App_typed with (τ1 := TUnit).
+  change ([TUnit] ++ Γ ⊢ₙₒ (FixArrow (FixLamBodyHelp e)).[ren (+1)] : TArrow TUnit τ). apply context_weakening.
+  apply FixArrow_typed. apply FixLamBodyHelp_typed. auto. by econstructor. constructor.
+Qed.
+
+Lemma FixLam_subst e σ : (FixLam e).[σ] = FixLam e.[up σ].
+Proof. rewrite /FixLam. by asimpl. Qed.
+
+Global Opaque FixLam.
+Global Opaque FixArrow.
