theories/lam/types.v
@@ -1,4 +1,4 @@
-From st Require Export autosubst.
+From st.prelude Require Import autosubst generic.
 
 Inductive type :=
  | TUnit : type
@@ -8,22 +8,24 @@ Inductive type :=
  | TSum (τ1 τ2 : type) : type
  | TArrow (τ1 τ2 : type) : type
  | TRec (τ : {bind 1 of type})
- | TVar (X : var)
- | TForall (τ : {bind 1 of type}).
+ | TVar (X : var).
+ (* | TForall (τ : {bind 1 of type}). *)
 
 Global Instance type_eq_dec (τ τ' : type) : Decision (τ = τ').
 Proof. solve_decision. Defined.
+
+Instance TVar_Inj : Inj eq eq TVar. intros x1 x2 eq. by inversion eq. Qed.
 
 Instance Ids_type : Ids type. derive. Defined.
 Instance Rename_type : Rename type. derive. Defined.
 Instance Subst_type : Subst type. derive. Defined.
 Instance SubstLemmas_typer : SubstLemmas type. derive. Qed.
 
-Declare Scope types_nost_scope.
+Declare Scope types_no_st_scope.
 
 Infix "×" := TProd (at level 49) : types_no_st_scope.
 Infix "+" := TSum : types_no_st_scope.
-Infix "⟶" := TArrow (at level 51) : types_no_st_scope.
+Infix "⟶" := TArrow (at level 51,right associativity) : types_no_st_scope.
 
 Delimit Scope types_no_st_scope with Tₙₒ.
 
@@ -35,3 +37,20 @@ Proof. by simpl. Qed.
 
 (* Lemma test'' : (TVar 0).[TVar 0/].[TInt/] = (TVar 0).[TVar 0,TInt/]. *)
 (* Proof. simpl. Qed. *)
+
+Lemma TVar_subst_list_closed_n_length (τs : list type) (X : var) (p : Closed_n (length τs) (TVar X)) :
+  (exists τ : type, τs !! X = Some τ ∧ (TVar X).[subst_list τs] = τ).
+Proof.
+  destruct (τs !! X) eqn:eq. exists t. split; auto. by apply ids_subst_list_lookup.
+  assert (length τs ≤ X). by apply lookup_ge_None.
+  assert (X < length τs). by apply ids_lt_Closed_n. lia.
+Qed.
+
+Inductive type_constructor :=
+  | TCUnit
+  | TCBool
+  | TCInt
+  | TCProd
+  | TCSum
+  | TCArrow
+  | TCRec.
