theories/prelude/autosubst.v
@@ -1,11 +1,11 @@
-From stdpp Require Export prelude.
-From iris Require Export prelude.
+From stdpp Require Import prelude.
+From iris Require Import prelude.
 From Autosubst Require Export Autosubst.
 
 Section Autosubst_Lemmas.
   Context {term : Type} {Ids_term : Ids term}
           {Rename_term : Rename term} {Subst_term : Subst term}
-          {SubstLemmas_term : SubstLemmas term}.
+          {SubstLemmas_term : SubstLemmas term} {ids_inj : Inj (=) (=) Ids_term}.
 
   Lemma iter_up (m x : nat) (f : var → term) :
     upn m f x = if lt_dec x m then ids x else rename (+m) (f (x - m)).
@@ -13,7 +13,6 @@ Section Autosubst_Lemmas.
     revert x; induction m as [|m IH]=> -[|x];
       repeat (destruct (lt_dec _ _) || asimpl || rewrite IH); auto with lia.
   Qed.
-
 
   Lemma iter_up_cases k n σ : (upn n σ k = ids k ∧ k < n) +
                                    { j : nat | (k = (n + j)%nat) ∧ upn n σ k = (σ j).[ren (+n)]  }.
@@ -37,18 +36,102 @@ Section Autosubst_Lemmas.
   Definition Closed_n (n : nat) (t : term) : Prop := ∀ σ, t.[upn n σ] = t.
   Definition Closed : term → Prop := Closed_n 0.
 
-  Definition subst_list (vs : list term) : var → term :=
+  Lemma ids_subst_yes n m σ : (ids (n + m)).[upn n σ] = ((ids m).[σ].[ren (+n)]).
+  Proof.
+    asimpl.
+    induction n.
+    - by asimpl.
+    - asimpl. rewrite IHn. by asimpl.
+  Qed.
+
+  Lemma ids_subst_no n m σ : n < m → (ids n).[upn m σ] = ids n.
+  Proof.
+    generalize dependent n.
+    induction m.
+    - intros. exfalso. lia.
+    - intros. destruct n.
+      + by asimpl.
+      + asimpl. specialize (IHm n). asimpl in IHm. rewrite IHm. by asimpl. lia.
+  Qed.
+
+  Lemma ids_subst_cases k n σ : ((ids k).[upn n σ] = ids k ∧ k < n) +
+                                  { j : nat | (k = (n + j)%nat) ∧ (ids k).[upn n σ] = (ids j).[σ].[ren (+n)]  }.
+  Proof.
+    destruct (decide (k < n)).
+    - apply inl. split. apply ids_subst_no; auto. auto.
+    - apply inr. exists (k - n). split. lia. rewrite -ids_subst_yes.
+      assert (triv : k = n + (k - n)). lia. by rewrite -triv.
+  Qed.
+
+  Lemma ids_lt_Closed_n (x n : nat) : Closed_n n (ids x) ↔ x < n.
+  Proof.
+    split.
+    - intros.
+      destruct (ids_subst_cases x n (ren (+1))) as [[_ eq] | [j [-> _]]].
+      + auto.
+      + exfalso. unfold Closed_n in H.
+        specialize (H (ren (+1))).
+        rewrite ids_subst_yes in H.
+        asimpl in H. assert (S (n + j) = n + j). by apply (inj ids). lia.
+    - intros. intro σ. by apply ids_subst_no.
+  Qed.
+
+  Definition subst_list_old (vs : list term) : var → term :=
     fun (x : var) => from_option id (ids x) (vs !! x).
 
-  Lemma simul_subst_closed (s t1 t2 : term) (Ct1 : Closed t1) (Ct2 : Closed t2) : s.[t1/].[t2/] = s.[t1,t2/].
-  Proof. asimpl. by rewrite Ct1. Qed.
+  Fixpoint subst_list (vs : list term) : var → term :=
+    match vs with
+    | [] => ids
+    | v :: vs' => v .: subst_list vs'
+    end.
 
-  Lemma scomp_closed_term (t : term) (Ct : Closed t) σ : t .: σ = t .: ids >> σ.
+  (* Lemma simul_subst_closed (s t1 t2 : term) (Ct1 : Closed t1) (Ct2 : Closed t2) : s.[t1/].[t2/] = s.[t1,t2/]. *)
+  (* Proof. asimpl. by rewrite Ct1. Qed. *)
+
+  (* Lemma scomp_closed_term (t : term) (Ct : Closed t) σ : t .: σ = t .: ids >> σ. *)
+  (* Proof. *)
+  (*   f_ext. intro x. induction x. *)
+  (*   - by simpl. *)
+  (*   - by asimpl. *)
+  (* Qed. *)
+
+  Lemma ids_subst_list_lookup (x : var) (ts : list term) t (H : ts !! x = Some t) :
+    (ids x).[subst_list ts] = t.
   Proof.
-    f_ext. intro x. induction x.
-    - by simpl.
-    - by asimpl.
+    generalize dependent x.
+    induction ts. intros. inversion H.
+    destruct x. intro H. inversion_clear H. by asimpl.
+    intro H. simpl in H. specialize (IHts _ H). by asimpl in *.
   Qed.
+
+  Lemma ids_subst_list_lookup2 (x : var) (ts : list term) :
+    (exists t, ts !! x = Some t ∧ (ids x).[subst_list ts] = t) ∨ (ts !! x = None).
+  Proof.
+    destruct (ts !! x) eqn:eq.
+    + left. exists t. split; auto. by apply ids_subst_list_lookup.
+    + right; auto.
+  Qed.
+
+  Lemma ids_subst_list_lt_length (x : var) (ts : list term) (p : x < length ts) :
+    (exists t, ts !! x = Some t ∧ (ids x).[subst_list ts] = t).
+  Proof.
+    destruct (ts !! x) eqn:eq. exists t. split; auto. by apply ids_subst_list_lookup.
+    assert (p' : length ts ≤ x). by apply lookup_ge_None. lia.
+  Qed.
+
+  (* Lemma subst_list_alt_cons_closed_S_n_type (t : term) (ts : list term) *)
+  (*       (tn : term) (Ctn : Closed_n (S (length ts)) tn) : *)
+  (* tn.[subst_list (t :: ts)] = tn.[up (subst_list ts)].[t/]. *)
+  (* Proof. by asimpl. Qed. *)
+
+(* Lemma subst_list_same vs : subst_list vs = subst_list_seq vs. *)
+  (* Proof. *)
+  (*   induction vs. *)
+  (*   asimpl. f_ext. intro y. by asimpl. *)
+  (*   asimpl. f_ext. intro y. asimpl. *)
+  (*   destruct y. by asimpl. asimpl. destruct (vs !! y) eqn:eq. *)
+  (*   asimpl. admit. simpl. asimpl. *)
+
 
   (* Lemma n_closed_invariant n (e : term) s1 s2 : *)
   (*   Closed_n n e → (∀ x, x < n → s1 x = s2 x) → e.[s1] = e.[s2]. *)
@@ -71,3 +154,11 @@ Section Autosubst_Lemmas.
   (* Qed. *)
 
 End Autosubst_Lemmas.
+
+Ltac closed_solver :=
+  lazymatch goal with
+  | H : Closed_n _ _ |- Closed_n _ _ => intros σ; specialize (H σ); simpl in H; by simplify_eq
+  | |- Closed_n _ _ => fail "goal detected suc"
+  | _ => fail "wrong goal"
+  end.
+
