theories/backtranslations/un_syn/expressions.v
@@ -1,0 +1,34 @@
+From st.lam Require Import lang lib.universe.base types.
+
+Reserved Notation "<< e >>" (at level 4, e at next level).
+Fixpoint back_expr (e : expr) : expr :=
+  match e with
+  | Var x => x
+  | LetIn e1 e2 => LetIn <<e1>> <<e2>>
+  | Lam e => inject TCArrow (Lam <<e>>)
+  (* | Fix e => Fix (extract TCArrow <<e>>) *)
+  | App e1 e2 => extract TCArrow <<e1>> <<e2>>
+  | Lit l => match l with
+            | LitInt n => inject TCInt n
+            | LitBool b => inject TCBool b
+            | LitUnit => inject TCUnit LitUnit
+            end
+  | BinOp op e1 e2 => inject (match op with
+                             | PlusOp => TCInt
+                             | MinusOp => TCInt
+                             | LeOp => TCBool
+                             | LtOp => TCBool
+                             | EqOp => TCBool
+                             end) (BinOp op (extract TCInt <<e1>>) (extract TCInt <<e2>>))
+  | If e0 e1 e2 => If (extract TCBool <<e0>>) <<e1>> <<e2>>
+  | Seq e1 e2 => Seq (extract TCUnit <<e1>>) <<e2>>
+  | Pair e1 e2 => inject TCProd (Pair <<e1>> <<e2>>)
+  | Fst e => Fst (extract TCProd <<e>>)
+  | Snd e => Snd (extract TCProd <<e>>)
+  | InjL e => inject TCSum (InjL <<e>>)
+  | InjR e => inject TCSum (InjR <<e>>)
+  | Case e0 e1 e2 => Case (extract TCSum <<e0>>) <<e1>> <<e2>>
+  | Fold e => inject TCRec (Fold <<e>>)
+  | Unfold e => Unfold (extract TCRec <<e>>)
+  end
+where "<< e >>" := (back_expr e).
