theories/backtranslations/un_syn/logrel/definitions.v
@@ -1,0 +1,98 @@
+From iris Require Import program_logic.weakestpre.
+From iris.proofmode Require Import tactics.
+From st.lam Require Import lang wkpre generic.lift types lib.universe.base.
+From st.backtranslations.un_syn Require Import expressions.
+
+Inductive refinement :=
+  | syn_le_un (* syntactically-typed in universe ≤ untyped *)
+  | un_le_syn. (* untyped ≤ syntactically-typed in universe *)
+
+Existing Class refinement.
+
+Section definitions.
+
+  Context `{Σ : !gFunctors}.
+  Context `{irisG_inst : !irisG lam_lang Σ}.
+
+  Context {rfn : refinement}.
+
+  Definition s : stuckness :=
+    match rfn with
+    | syn_le_un => NotStuck
+    | un_le_syn => MaybeStuck (* untyped can of course get stuck *)
+    end.
+
+  Definition canon_tc_lift (tc : type_constructor) (Ψ : valO -n> valO -n> iPropO Σ) (xᵢ xₛ : valO) : iPropO Σ :=
+    (match tc with
+     | TCUnit => ⌜ xᵢ = ()%Vₙₒ ⌝ ∧ ⌜ xₛ = ()%Vₙₒ ⌝
+     | TCBool => ∃ b : bool, ⌜ xᵢ = b%Vₙₒ ⌝ ∧ ⌜ xₛ = b ⌝
+     | TCInt => ∃ z : Z, ⌜ xᵢ = z%Vₙₒ ⌝ ∧ ⌜ xₛ = z ⌝
+     | TCProd => ∃ v1 v2 v1' v2', ⌜ xᵢ = (v1, v2)%Vₙₒ ⌝ ∧ ⌜ xₛ = (v1', v2')%Vₙₒ ⌝ ∧ (▷ Ψ v1 v1') ∗ (▷ Ψ v2 v2')
+     | TCSum => ∃ vi vi', (⌜ xᵢ = InjLV vi ⌝ ∧ ⌜ xₛ = InjLV vi' ⌝ ∧ ▷ Ψ vi vi') ∨
+                         (⌜ xᵢ = InjRV vi ⌝ ∧ ⌜ xₛ = InjRV vi' ⌝ ∧ ▷ Ψ vi vi')
+     | TCArrow => ∃ e e', ⌜ xᵢ = LamV e ⌝ ∧ ⌜ xₛ = LamV e' ⌝ ∧ ▷ □ (∀ w w', Ψ w w' -∗ lift s Ψ e.[of_val w/] e'.[of_val w'/])
+     | TCRec => ∃ w w', ⌜ xᵢ = FoldV w ⌝ ∧ ⌜ xₛ = FoldV w' ⌝ ∧ ▷ Ψ w w'
+     end)%I.
+
+  Definition valrel_gen_pre (Ψ : valO -n> valO -n> iPropO Σ) (vᵢ vₛ : valO) : iPropO Σ :=
+    match rfn with
+    | syn_le_un => (∃ tc vᵢ', ⌜ vᵢ = inject_val tc vᵢ' ⌝ ∧ canon_tc_lift tc Ψ vᵢ' vₛ)%I
+    | un_le_syn => (∃ tc vₛ', ⌜ vₛ = inject_val tc vₛ' ⌝ ∧ canon_tc_lift tc Ψ vᵢ vₛ')%I
+    end.
+
+  Definition valrel_gen (Ψ : valO -n> valO -n> iPropO Σ) : valO -n> valO -n> iPropO Σ := λne v v', valrel_gen_pre Ψ v v'.
+
+  Instance valrel_gen_contractive : Contractive valrel_gen.
+  Proof.
+    intros n P1 P2 dl. rewrite /valrel_gen. intros v v'. simpl.
+    rewrite /valrel_gen_pre; destruct rfn; f_equiv; intro tc; rewrite /inject_val /InjVTC /canon_tc_lift; destruct tc; rewrite /lift; solve_contractive.
+  Qed.
+
+  Definition valrel := fixpoint valrel_gen.
+
+  Lemma valrel_unfold v1 v2 : fixpoint valrel_gen v1 v2 ≡ valrel_gen (fixpoint valrel_gen) v1 v2.
+  Proof. do 2 f_equiv. by rewrite -fixpoint_unfold. Qed.
+
+  Global Instance valrel_persistent u v' : Persistent (valrel u v').
+  Proof.
+    rewrite /Persistent. revert u v'. iLöb as "IHlob". iIntros (u v') "Huv'".
+    rewrite valrel_unfold /= /valrel_gen_pre. destruct rfn.
+    { iDestruct "Huv'" as (tc v) "[-> Hvv']".
+    iExists tc, v. iSplit; auto. destruct tc; try by iDestruct "Hvv'" as "#Hvv'".
+    - simpl; fold valrel. iDestruct "Hvv'" as (v1 v2 v1' v2') "(-> & -> & H1 & H2)".
+      iExists v1, v2, v1', v2'. repeat iSplit; auto.
+      iApply bi.later_persistently_1. iNext. by iApply "IHlob".
+      iApply bi.later_persistently_1. iNext. by iApply "IHlob".
+    - simpl; fold valrel. iDestruct "Hvv'" as (vi vi') "[(-> & -> & H) | (-> & -> & H)]".
+      iExists _, _. iLeft. repeat iSplit; auto. iApply bi.later_persistently_1. by iApply "IHlob".
+      iExists _, _. iRight. repeat iSplit; auto. iApply bi.later_persistently_1. by iApply "IHlob".
+    - simpl. fold valrel. iDestruct "Hvv'" as (w w') "(-> & -> & H)".
+      iExists _,_. repeat iSplit; auto. iApply bi.later_persistently_1. by iApply "IHlob". }
+    { iDestruct "Huv'" as (tc v) "[-> Hvv']".
+    iExists tc, v. iSplit; auto. destruct tc; try by iDestruct "Hvv'" as "#Hvv'".
+    - simpl; fold valrel. iDestruct "Hvv'" as (v1 v2 v1' v2') "(-> & -> & H1 & H2)".
+      iExists v1, v2, v1', v2'. repeat iSplit; auto.
+      iApply bi.later_persistently_1. iNext. by iApply "IHlob".
+      iApply bi.later_persistently_1. iNext. by iApply "IHlob".
+    - simpl; fold valrel. iDestruct "Hvv'" as (vi vi') "[(-> & -> & H) | (-> & -> & H)]".
+      iExists _, _. iLeft. repeat iSplit; auto. iApply bi.later_persistently_1. by iApply "IHlob".
+      iExists _, _. iRight. repeat iSplit; auto. iApply bi.later_persistently_1. by iApply "IHlob".
+    - simpl. fold valrel. iDestruct "Hvv'" as (w w') "(-> & -> & H)".
+      iExists _,_. repeat iSplit; auto. iApply bi.later_persistently_1. by iApply "IHlob". }
+  Qed.
+
+  Definition exprel : exprO -n> exprO -n> iPropO Σ :=
+    λne eᵢ eₛ, lift s valrel eᵢ eₛ.
+
+  Definition closed_condition n (e e' : expr) : Prop :=
+    Closed_n n match rfn with
+               | syn_le_un => e'
+               | un_le_syn => e
+               end.
+
+  Definition open_exprel (n : nat) (e e' : expr) (pne' : closed_condition n e e') : Prop :=
+    ∀ (us : list val) (vs' : list val), length us = n →
+      ([∗ list] uᵢ ; vᵢ' ∈ us ; vs', valrel uᵢ vᵢ') ⊢
+        exprel e.[subst_list_val us] e'.[subst_list_val vs'].
+
+End definitions.
