theories/lam/lib/dummy.v
@@ -1,4 +1,4 @@
-From st.lam Require Export lang.
+From st.lam Require Import lang.
 
 Definition dummy : expr.
 Proof. exact ()%Eₙₒ. Qed.
