theories/lam/lib/guard_assert.v
@@ -1,0 +1,140 @@
+From st.prelude Require Import autosubst.
+From st.lam Require Import types lang typing tactics.
+From st.lam.lib Require Import fixlam omega universe.base dummy.
+
+Inductive action :=
+  | Guard
+  | Assert.
+
+Definition FstSndga (ga : action) : expr → expr :=
+  match ga with
+  | Guard => Fst
+  | Assert => Snd
+  end.
+
+Definition opp_action (ga : action) :=
+  match ga with
+  | Guard => Assert
+  | Assert => Guard
+  end.
+
+Definition fixgenTRecga (gb ab : val) : val :=
+  (LamV (* 1 → ((τ → τ) × (τ → τ)) *) (
+       LamV (* 1 *) (
+           ( LamV (Fold (gb.{ren (+2)} (Unfold %0))) , (* τ → τ *)
+             LamV (Fold (ab.{ren (+2)} (Unfold %0))) (* τ → τ *)
+           )
+         )
+     )
+  )%Eₙₒ.
+
+Lemma fixgenTRecga_subst (gb ab : val) (σ : var → expr) : (fixgenTRecga gb ab).{σ} = fixgenTRecga gb.{up σ} ab.{up σ}.
+Proof. rewrite /fixgenTRecga. repeat rewrite -val_subst_valid. by asimpl. Qed.
+
+(* Lemma App_fixgenTRecga_lam_step (gb ab : val) (e : expr) : *)
+(*   lam_step (fixgenTRecga gb ab (Lam e)) *)
+(* ((LamV ( *)
+(*            ( LamV (Fold ((of_val gb).[Lam e.[ren (0 .: (+3))] .: ren (+2)] (Unfold %0))) , (* τ → τ *) *)
+(*              LamV (Fold ((of_val ab).[Lam e.[ren (0 .: (+3))] .: ren (+2)] (Unfold %0))) (* τ → τ *) *)
+(*            ) *)
+(*          )))%Eₙₒ. *)
+(* Proof. *)
+(*   assert ( *)
+(* (of_val (LamV ( *)
+(*            ( LamV (Fold ((of_val gb).[Lam e.[ren (0 .: (+3))] .: ren (+2)] (Unfold %0))) , (* τ → τ *) *)
+(*              LamV (Fold ((of_val ab).[Lam e.[ren (0 .: (+3))] .: ren (+2)] (Unfold %0))) (* τ → τ *) *)
+(*            ) *)
+(*          )))%Eₙₒ = *)
+(* ((LamV ( *)
+(*            ( LamV (Fold ((of_val gb).[ren (+2)] (Unfold %0))) , (* τ → τ *) *)
+(*              LamV (Fold ((of_val ab).[ren (+2)] (Unfold %0))) (* τ → τ *) *)
+(*            ) *)
+(*          )))%Eₙₒ.[Lam e/] *)
+(*     ) as ->. by asimpl. *)
+(*   apply head_prim_step. eapply App_Lam_head_step. by simpl. *)
+(* Qed. *)
+
+Lemma fixgenTRecga_typed (gb ab : val) Γ τb
+      (pgb : (TUnit ⟶ ((TRec τb ⟶ TRec τb) × (TRec τb ⟶ TRec τb)))%Tₙₒ :: Γ ⊢ₙₒ gb : τb.[TRec τb/] ⟶ τb.[TRec τb/])
+      (pab : (TUnit ⟶ ((TRec τb ⟶ TRec τb) × (TRec τb ⟶ TRec τb)))%Tₙₒ :: Γ ⊢ₙₒ ab : τb.[TRec τb/] ⟶ τb.[TRec τb/]) :
+  Γ ⊢ₙₒ fixgenTRecga gb ab :
+    (TUnit ⟶ ((TRec τb ⟶ TRec τb) × (TRec τb ⟶ TRec τb))) ⟶ (TUnit ⟶ ((TRec τb ⟶ TRec τb) × (TRec τb ⟶ TRec τb))).
+Proof.
+  constructor. constructor. constructor.
+  constructor. constructor. apply App_typed with (τ1 := τb.[TRec τb/]). rewrite -val_subst_valid.
+  apply context_weakening2. apply pgb.
+  constructor. by constructor.
+  constructor. constructor. apply App_typed with (τ1 := τb.[TRec τb/]). rewrite -val_subst_valid.
+  apply context_weakening2. apply pab.
+  constructor. by constructor.
+Qed.
+
+Global Opaque fixgenTRecga.
+
+(* Lemma test (t : expr) : t = (ids 1).[up (ren (+2))]. *)
+(* asimpl.  *)
+Fixpoint ga_pair (ga : action) (τ : type) : val :=
+  (match τ with
+   | TUnit => match ga with
+             | Guard => LamV %0
+             | Assert => LamV (Seq %0 ())
+             end
+   | TBool => match ga with
+             | Guard => LamV %0
+             | Assert => LamV (If %0 true false)
+             end
+   | TInt => match ga with
+            | Guard => LamV %0
+            | Assert => LamV (%0 + 0)
+            end
+   | TProd τ1 τ2 => LamV (LetIn (Fst %0) (LetIn (Snd %1) ((ga_pair ga τ1).{ren (+3)} %1, (ga_pair ga τ2).{ren (+3)} %0)))
+   | TSum τ1 τ2 => LamV (Case %0 (InjL ((ga_pair ga τ1).{ren (+2)} %0)) (InjR ((ga_pair ga τ2).{ren (+2)} %0)))
+   | TArrow τ1 τ2 => LamV (Lam ((ga_pair ga τ2).{ren (+2)} (%1 ((ga_pair (opp_action ga) τ1).{ren (+2)} %0))))
+   | TRec τb => let β := fixgenTRecga (ga_pair Guard τb) (ga_pair Assert τb) in
+               LamV (FstSndga ga (LamV (FixArrow β.{ren (+2)} %0(*_*)) ()) %0)
+   | TVar X => LamV (FstSndga ga (Var (S X) ()) %0)
+   end)%Eₙₒ.
+
+(* We never actually need typedness of ga; but it serves as a good sanity check *)
+Lemma ga_typed_gen (τ : type) (τs : list type) (pτn : Closed_n (length τs) τ) (ga : action) :
+  map (fun τ => (TUnit ⟶ (τ ⟶ τ) × (τ ⟶ τ))%Tₙₒ) τs ⊢ₙₒ (ga_pair ga τ) : (τ.[subst_list τs] ⟶ τ.[subst_list τs]).
+Proof.
+  generalize dependent ga.
+  generalize dependent τs.
+  induction τ as [ | | | τ1 IHτ1 τ2 IHτ2 | τ1 IHτ1 τ2 IHτ2 | τ1 IHτ1 τ2 IHτ2 | τb IHτb | X ]; intros τs Cnτ ga;
+    try by (destruct ga; by repeat econstructor).
+  - repeat econstructor; fold ga_pair.
+    rewrite -val_subst_valid. apply context_weakening3. apply IHτ1. closed_solver.
+    rewrite -val_subst_valid. apply context_weakening3. apply IHτ2. closed_solver.
+  - repeat econstructor; fold ga_pair.
+    rewrite -val_subst_valid. apply context_weakening2. apply IHτ1. closed_solver.
+    rewrite -val_subst_valid. apply context_weakening2. apply IHτ2. closed_solver.
+  - repeat econstructor; fold ga_pair.
+    rewrite -val_subst_valid. apply context_weakening2. apply IHτ2. closed_solver.
+    rewrite -val_subst_valid. apply context_weakening2. apply IHτ1. closed_solver.
+  - (* TRec *) destruct ga.
+    + constructor. fold ga_pair.
+      apply App_typed with (τ1 := (TRec τb).[subst_list τs]). 2: by constructor.
+      eapply Fst_typed.
+      apply App_typed with (τ1 := TUnit). 2: by constructor. apply Lam_typed.
+      apply App_typed with (τ1 := TUnit). 2: by constructor.
+      apply FixArrow_typed. rewrite -val_subst_valid. apply context_weakening2. apply fixgenTRecga_typed.
+      * asimpl. change (TRec τb.[up (subst_list τs)] .: subst_list τs) with (subst_list (TRec τb.[up (subst_list τs)] :: τs)).
+        rewrite -map_cons. apply IHτb with (ga := Guard). closed_solver.
+      * asimpl. change (TRec τb.[up (subst_list τs)] .: subst_list τs) with (subst_list (TRec τb.[up (subst_list τs)] :: τs)).
+        rewrite -map_cons. apply IHτb with (ga := Assert). closed_solver.
+    + constructor. fold ga_pair.
+      eapply App_typed. 2: by constructor.
+      eapply Snd_typed.
+      apply App_typed with (τ1 := TUnit). 2: by constructor. apply Lam_typed.
+      apply App_typed with (τ1 := TUnit). 2: by constructor.
+      apply FixArrow_typed. rewrite -val_subst_valid. apply context_weakening2.
+      simpl. apply fixgenTRecga_typed.
+      * asimpl. change (TRec τb.[up (subst_list τs)] .: subst_list τs) with (subst_list (TRec τb.[up (subst_list τs)] :: τs)).
+        rewrite -map_cons. apply IHτb with (ga := Guard). closed_solver.
+      * asimpl. change (TRec τb.[up (subst_list τs)] .: subst_list τs) with (subst_list (TRec τb.[up (subst_list τs)] :: τs)).
+        rewrite -map_cons. apply IHτb with (ga := Assert). closed_solver.
+  - (* TVar *)
+    destruct (TVar_subst_list_closed_n_length _ _ Cnτ) as [τ [eq ->]].
+    destruct ga; repeat econstructor; simpl; by rewrite list_lookup_fmap eq /=.
+Qed.
