theories/lam/lib/omega.v
@@ -1,13 +1,32 @@
-From st.lam Require Export types lang typing.
+From st.lam Require Import types lang typing tactics.
 
 Definition Ω : expr :=
-  (Rec (%0 %1) ())%Eₙₒ.
+  (Lam (Unfold %0 %0)
+       (Fold (Lam (Unfold %0 %0)))
+  )%Eₙₒ.
+  (* (Fix (Lam %0))%Eₙₒ. *)
+  (* (Rec (%0 %1) ())%Eₙₒ. *)
 
-Lemma Ω_loop σ κ : prim_step Ω σ κ Ω σ [].
-Proof. apply head_prim_step. rewrite /Ω. by eapply BetaS. Qed.
+Lemma Ω_Closed : Closed Ω.
+Proof. intro σ. by asimpl. Qed.
 
 Lemma Ω_typed Γ τ : Γ ⊢ₙₒ Ω : τ.
 Proof.
-  rewrite /Ω. eapply App_typed; try by constructor.
-  apply Rec_typed. eapply App_typed; by constructor.
+  apply App_typed with (τ1 := TRec (TVar 0 ⟶ τ.[ren (+1)])%Tₙₒ).
+  apply Lam_typed. apply App_typed with (τ1 := TRec (TVar 0 ⟶ τ.[ren (+1)])%Tₙₒ). assert ((TRec (TVar 0 ⟶ τ.[ren (+1)]) ⟶ τ)%Tₙₒ = (TVar 0 ⟶ τ.[ren (+1)])%Tₙₒ.[TRec (TVar 0 ⟶ τ.[ren (+1)])%Tₙₒ/]) as ->. by asimpl. do 3 econstructor.
+  by econstructor. econstructor. asimpl.
+  apply Lam_typed. apply App_typed with (τ1 := TRec (TVar 0 ⟶ τ.[ren (+1)])%Tₙₒ). assert ((TRec (TVar 0 ⟶ τ.[ren (+1)]) ⟶ τ)%Tₙₒ = (TVar 0 ⟶ τ.[ren (+1)])%Tₙₒ.[TRec (TVar 0 ⟶ τ.[ren (+1)])%Tₙₒ/]) as ->. by asimpl. do 3 econstructor.
+  by econstructor.
 Qed.
+
+Lemma Ω_loop : nsteps lam_step 2 Ω Ω.
+Proof. do 2 (eapply nsteps_l; first auto_lam_step; simpl). by apply nsteps_O. Qed.
+
+(* From st.lam Require Import wkpre. *)
+(* From iris Require Import program_logic.weakestpre. *)
+(* From iris.proofmode Require Import tactics. *)
+
+(* Lemma wp_Ω Φ : ⊢ WP Ω {{Φ}}. *)
+(* Proof. iLöb as "IH". iApply wp_steps_later. by apply Ω_loop. done. Qed. *)
+
+Global Opaque Ω.
