theories/lam/logrel/definitions.v
@@ -1,0 +1,79 @@
+From iris Require Import program_logic.weakestpre.
+From iris.proofmode Require Import tactics.
+From st.lam Require Import lang types wkpre generic.lift.
+
+Canonical Structure typeO := leibnizO type.
+
+Section definition.
+
+  Context `{Σ : !gFunctors}.
+  Context `{irisG_inst : !irisG lam_lang Σ}.
+
+  (* We define a stuckness-sensistive and insensitive one *)
+  Context (s : stuckness).
+
+  Fixpoint valrel_typed_gen_pre (Ψ : typeO -n> valO -n> valO -n> iPropO Σ) (τ : typeO) : valO -n> valO -n> iPropO Σ := λne v v',
+    (match τ with
+     | TUnit => ⌜ v = (()%Vₙₒ : valO) ⌝ ∧ ⌜ v' = (()%Vₙₒ : valO) ⌝
+     | TBool => ∃ b : bool, ⌜ v = b ⌝ ∧ ⌜ v' = b ⌝
+     | TInt => ∃ z : Z, ⌜ v = z ⌝ ∧ ⌜ v' = z ⌝
+     | TProd τ1 τ2 => ∃ v1 v2 v1' v2', ⌜ v = (v1, v2)%Vₙₒ ⌝ ∧ ⌜ v' = (v1' , v2')%Vₙₒ ⌝ ∗ valrel_typed_gen_pre Ψ τ1 v1 v1' ∗ valrel_typed_gen_pre Ψ τ2 v2 v2'
+     | TSum τ1 τ2 => ∃ vi vi', (⌜ v = InjLV vi ⌝ ∧ ⌜ v' = InjLV vi' ⌝ ∧ valrel_typed_gen_pre Ψ τ1 vi vi') ∨
+                              (⌜ v = InjRV vi ⌝ ∧ ⌜ v' = InjRV vi' ⌝ ∧ valrel_typed_gen_pre Ψ τ2 vi vi')
+     | TArrow τ1 τ2 => □ (∀ w w', valrel_typed_gen_pre Ψ τ1 w w' -∗ lift s (valrel_typed_gen_pre Ψ τ2) (v w) (v' w'))
+     | TRec τ => ∃ w w', ⌜ v = FoldV w ⌝ ∧ ⌜ v' = FoldV w' ⌝ ∧ ▷ (Ψ τ.[TRec τ/] w w')
+     | TVar X => False
+     end)%I.
+
+  Definition valrel_typed_gen (Ψ : typeO -n> valO -n> valO -n> iPropO Σ) : typeO -n> valO -n> valO -n> iPropO Σ := λne τ v v', valrel_typed_gen_pre Ψ τ v v'.
+
+  Instance valrel_typed_gen_contractive : Contractive valrel_typed_gen.
+  Proof.
+    intros n P1 P2 dl. rewrite /valrel_typed_gen. intro τ. simpl.
+    induction τ; try by solve_contractive.
+    - intros v v'. simpl. do 6 f_equiv. specialize (IHτ1 a a0). simpl in IHτ1. by rewrite IHτ1.
+      rewrite /lift. do 5 f_equiv. specialize (IHτ2 a1 a2). simpl in IHτ2. by rewrite IHτ2.
+  Qed.
+
+  Definition valrel_typed := fixpoint valrel_typed_gen.
+
+  Lemma valrel_typed_unfold τ v1 v2 : valrel_typed τ v1 v2 ≡ valrel_typed_gen (fixpoint valrel_typed_gen) τ v1 v2.
+  Proof. do 3 f_equiv. by rewrite -fixpoint_unfold. Qed.
+  Lemma valrel_typed_unfold' τ : valrel_typed τ ≡ valrel_typed_gen (fixpoint valrel_typed_gen) τ.
+  Proof. intros x x'. by rewrite valrel_typed_unfold. Qed.
+  Lemma valrel_typed_unfold'' : valrel_typed ≡ valrel_typed_gen (fixpoint valrel_typed_gen).
+  Proof. intros x. by rewrite valrel_typed_unfold'. Qed.
+  Lemma valrel_typed_gen_pre_gen Ψ τ v v' : valrel_typed_gen_pre Ψ τ v v' ≡ valrel_typed_gen Ψ τ v v'.
+  Proof. auto. Qed.
+  Lemma valrel_typed_gen_pre_gen' Ψ τ : valrel_typed_gen_pre Ψ τ ≡ valrel_typed_gen Ψ τ.
+  Proof. intro. intro. auto. Qed.
+  Lemma valrel_typed_TArrow_unfold τ1 τ2 v v' : valrel_typed (TArrow τ1 τ2) v v' ≡ (□ (∀ w w', valrel_typed τ1 w w' -∗ lift s (valrel_typed τ2) (v w) (v' w')))%I.
+  Proof.
+    rewrite valrel_typed_unfold. rewrite /valrel_typed_gen. simpl.
+    f_equiv. f_equiv. intros w. f_equiv. intro w'. f_equiv.
+    - rewrite valrel_typed_gen_pre_gen. unfold valrel_typed. rewrite -valrel_typed_unfold. auto.
+    - rewrite /lift. f_equiv. simpl. f_equiv. f_equiv. f_equiv. f_equiv.
+      by rewrite valrel_typed_unfold.
+  Qed.
+
+  Ltac simpl_valrel_typed := fold (valrel_typed_gen_pre); repeat rewrite valrel_typed_gen_pre_gen -valrel_typed_unfold; fold (valrel_typed).
+
+  Global Instance valrel_typed_persistent τ v v' : Persistent (valrel_typed τ v v').
+  Proof.
+    rewrite /Persistent. revert τ v v'. iLöb as "IHlob". iIntros (τ).
+    iInduction τ as [ | | | τ1 τ2 | τ1 τ2 | τ1 τ2 | τ1 τ2 | τ ] "IH";
+      iIntros (v v'); rewrite valrel_typed_unfold; try by iIntros "#H".
+    - iIntros "H". iDestruct "H" as (v1 v2 v1' v2') "(-> & -> & H1 & H2)". simpl_valrel_typed.
+      iExists v1, v2, v1', v2'. simpl_valrel_typed. repeat iSplit; auto. iApply ("IH" with "H1"). iApply ("IH1" with "H2").
+    - simpl_valrel_typed. iIntros "H". iDestruct "H" as (vi vi') "[(-> & -> & H1) | (-> & -> & H2)]"; iExists vi, vi'; simpl_valrel_typed.
+      + iLeft. repeat iSplit; auto. by iApply ("IH" with "H1").
+      + iRight. repeat iSplit; auto. by iApply ("IH1" with "H2").
+    - iIntros "H". iDestruct "H" as (w w') "(-> & -> & H)". simpl_valrel_typed. iExists w, w'. repeat iSplitL ""; auto.
+      iApply bi.later_persistently_1. iNext. by iApply "IHlob".
+  Qed.
+
+  Definition exprel_typed : typeO -n> exprO -n> exprO -n> iPropO Σ := λne τ eᵢ eₛ, lift s (valrel_typed τ) eᵢ eₛ.
+
+End definition.
+
+Ltac simpl_valrel_typed := fold (valrel_typed_gen_pre); repeat rewrite valrel_typed_gen_pre_gen -valrel_typed_unfold; fold (valrel_typed).
