theories/lam/tactics.v
@@ -1,0 +1,206 @@
+From st.lam Require Import lang.
+
+Fixpoint ectx_expr (e : expr) : list ectx_item :=
+  match e with
+  | Var x => []
+  | LetIn e1 e2 => match to_val e1 with
+                 | Some v1 => []
+                 | None =>  ectx_expr e1 ++ [LetInCtx e2]
+                 end
+  | Lam e => []
+  (* | Fix e => match to_val e with *)
+            (* | Some v => [] *)
+            (* | None => ectx_expr e ++ [FixCtx] *)
+            (* end *)
+  | App e1 e2 => match to_val e1 with
+                | Some v1 => match to_val e2 with
+                            | Some v2 => []
+                            | None => ectx_expr e2 ++ [AppRCtx v1]
+                         end
+                | None => ectx_expr e1 ++ [AppLCtx e2]
+                end
+  | Lit l => []
+  | BinOp op e1 e2 => match to_val e1 with
+                     | Some v1 => match to_val e2 with
+                                 | Some v2 => []
+                                 | None => ectx_expr e2 ++ [BinOpRCtx op v1]
+                                 end
+                     | None => ectx_expr e1 ++ [BinOpLCtx op e2]
+                     end
+  | If e0 e1 e2 => match to_val e0 with
+                  | Some v0 => []
+                  | None => ectx_expr e0 ++ [IfCtx e1 e2]
+                  end
+  | Seq e1 e2 => match to_val e1 with
+                | Some v1 => []
+                | None => ectx_expr e1 ++ [SeqCtx e2]
+                end
+  | Pair e1 e2 => match to_val e1 with
+                 | Some v1 => match to_val e2 with
+                             | Some v2 => []
+                             | None => ectx_expr e2 ++ [PairRCtx v1]
+                             end
+                 | None => ectx_expr e1 ++ [PairLCtx e2]
+                 end
+  | Fst e => match to_val e with
+            | Some v => []
+            | None => ectx_expr e ++ [FstCtx]
+            end
+  | Snd e => match to_val e with
+            | Some v => []
+            | None => ectx_expr e ++ [SndCtx]
+            end
+  | InjL e => match to_val e with
+             | Some v => []
+             | None => ectx_expr e ++ [InjLCtx]
+             end
+  | InjR e => match to_val e with
+             | Some v => []
+             | None => ectx_expr e ++ [InjRCtx]
+             end
+  | Case e0 e1 e2 => match to_val e0 with
+                    | Some v0 => []
+                    | None => ectx_expr e0 ++ [CaseCtx e1 e2]
+                    end
+  | Fold e => match to_val e with
+                | Some v => []
+                | None => ectx_expr e ++ [FoldCtx]
+                end
+  | Unfold e => match to_val e with
+                | Some v => []
+                | None => ectx_expr e ++ [UnfoldCtx]
+                end
+  (* | TLam e => [] *)
+  (* | TApp e => match to_val e with *)
+             (* | Some v => [] *)
+             (* | None => ectx_expr e ++ [TAppCtx] *)
+             (* end *)
+  end.
+
+
+Fixpoint head_expr (e : expr) : expr :=
+  match e with
+  | Var x => Var x
+  | LetIn e1 e2 => match to_val e1 with
+                 | Some v1 => LetIn v1 e2
+                 | None => head_expr e1
+                 end
+  | Lam e => LamV e
+  (* | Fix e => match to_val e with *)
+            (* | Some v => Fix v *)
+            (* | None => head_expr e *)
+            (* end *)
+  | App e1 e2 => match to_val e1 with
+                | Some v1 => match to_val e2 with
+                            | Some v2 => App v1 v2
+                            | None => head_expr e2
+                         end
+                | None => head_expr e1
+                end
+  | Lit l => LitV l
+  | BinOp op e1 e2 => match to_val e1 with
+                     | Some v1 => match to_val e2 with
+                                 | Some v2 => BinOp op v1 v2
+                                 | None => head_expr e2
+                                 end
+                     | None => head_expr e1
+                     end
+  | If e0 e1 e2 => match to_val e0 with
+                  | Some v0 => If v0 e1 e2
+                  | None => head_expr e0
+                  end
+  | Seq e1 e2 => match to_val e1 with
+                | Some v1 => Seq v1 e2
+                | None =>  head_expr e1
+                end
+  | Pair e1 e2 => match to_val e1 with
+                 | Some v1 => match to_val e2 with
+                             | Some v2 => Pair v1 v2
+                             | None => head_expr e2
+                             end
+                 | None => head_expr e1
+                 end
+  | Fst e => match to_val e with
+            | Some v => Fst v
+            | None => head_expr e
+            end
+  | Snd e => match to_val e with
+            | Some v => Snd v
+            | None => head_expr e
+            end
+  | InjL e => match to_val e with
+             | Some v => InjLV v
+             | None => head_expr e
+             end
+  | InjR e => match to_val e with
+             | Some v => InjRV v
+             | None => head_expr e
+             end
+  | Case e0 e1 e2 => match to_val e0 with
+                    | Some v0 => Case v0 e1 e2
+                    | None => head_expr e0
+                    end
+  | Fold e => match to_val e with
+                | Some v => FoldV v
+                | None => head_expr e
+                end
+  | Unfold e => match to_val e with
+                | Some v => Unfold v
+                | None => head_expr e
+                end
+  (* | TLam e => TLamV e *)
+  (* | TApp e => match to_val e with *)
+             (* | Some v => TApp v *)
+             (* | None => head_expr e *)
+             (* end *)
+  end.
+
+(* Lemma prim_step_pure e σ κ e' : prim_step e [] e' [] → pure_step e e'. *)
+(* Proof. *)
+(*   intro Hp. split. *)
+(*   + intro σ. destruct σ. exists e', tt, []. by simpl. *)
+(*   + intros. destruct σ1, σ2. simpl in H. *)
+(*     assert (efs = []) as ->; first by inversion H. assert (κ = []) as ->; first by inversion H. *)
+(*     erewrite (prim_step_det e e' e2'); eauto. *)
+(* Qed. *)
+
+
+Lemma split_expr (e : expr) : e = fill (ectx_expr e) (head_expr e).
+Proof.
+  induction e as [x | e1 IH1 e2 IH2 | e1 IH1 | e1 IH1 e2 IH2 | e1 | binop e1 IH1 e2 IH2 | e1 IH1 e2 IH2 e3 IH3 | e1 IH1 e2 IH2 | e1 IH1 e2 IH2 | e1 IH1 | e1 IH1 | e1 IH1 | e1 IH1 | e1 IH1 e2 IH2 | e1 IH1 | e1 IH1 ];
+    try done; repeat ((destruct (to_val e1) eqn:eq1 || destruct (to_val e2) eqn:eq2 || rewrite fill_app || rewrite (of_to_val _ _ eq1) || rewrite (of_to_val _ _ eq2) || rewrite eq1 || rewrite eq2 || rewrite -IH1 || rewrite -IH2 || simpl)); auto.
+Qed.
+
+Ltac simplify_custom := (simplify_option_eq; asimpl; (repeat (rewrite to_of_val /=; asimpl)); simplify_option_eq).
+
+Ltac auto_head_step :=
+  lazymatch goal with
+  | |- head_step _ _ _ _ _ _ => by (simplify_custom; econstructor; simplify_custom)
+  | |- ectx_language.head_step _ _ _ _ _ _ => by (simplify_custom; econstructor; simplify_custom)
+  | |- _ => fail "Goal not a head_step"
+  end.
+
+Ltac ectx_lam_step :=
+  lazymatch goal with
+  | |- lam_step ?e _ => eapply (Ectx_step (ectx_expr e) (head_expr e) _ (split_expr e)); first eauto
+  | |- _ => fail "Goal not a lam_step"
+  end.
+
+Ltac auto_lam_step :=
+  lazymatch goal with
+  | |- lam_step ?e _ => by (ectx_lam_step; auto_head_step)
+  | |- _ => fail "Goal not a lam_step"
+  end.
+
+Ltac auto_rtc_lam_step :=
+  lazymatch goal with
+  | |- rtc lam_step ?e ?e => by apply rtc_refl
+  | |- rtc lam_step _ _ => (eapply rtc_l; first (auto_lam_step); simplify_custom)
+  | |- _ => fail "Goal not a rtc lam_step"
+  end.
+
+
+(* Hint Extern 5 (IntoVal _ _) => eapply of_to_val; fast_done : typeclass_instances. *)
+(* Hint Extern 10 (IntoVal _ _) => *)
+(*   rewrite /IntoVal; eapply of_to_val; rewrite /= !to_of_val /=; solve [ eauto ] : typeclass_instances. *)
+
