theories/prelude/generic.v
@@ -1,0 +1,2 @@
+From stdpp Require Export prelude.
+From iris Require Export prelude.
